Introduce equation proxy for rules, solving all issues

theories/Env.v
@@ -8,8 +8,8 @@
 **)
 
 From Stdlib Require Import Utf8 String List Arith.
-From LocalComp.autosubst Require Import AST.
-From LocalComp Require Import BasicAST.
+From LocalComp.autosubst Require Import AST SubstNotations RAsimpl AST_rasimpl.
+From LocalComp Require Import Util BasicAST.
 
 Import ListNotations.
 
@@ -44,6 +44,14 @@ Definition ectx_get (Ξ : ectx) (M : eref) :=
 
 (** Custom computation rule
 
+  We consider them as definitional equalities which might be nonlinear.
+  For implementation purposes however, it's better to have a linear version
+  (as well as pattern syntax) so we consider the left-hand side as the result of
+  applying a "forcing" substitution.
+
+  To make the inlining proof easier and more general, we will consider an
+  equation proxy where the substitution is already applied.
+
   Fields are
   - [cr_env]: the environment of the rule [Θ]
   - [cr_pat]: the "pattern" for the left-hand side [p]
@@ -62,6 +70,21 @@ Record crule := {
   cr_rep : term ;
   cr_typ : term
 }.
+
+Record equation := {
+  eq_env : ctx ;
+  eq_lhs : term ;
+  eq_rhs : term ;
+  eq_typ : term
+}.
+
+Definition crule_eq rule : equation := {|
+  eq_env := rule.(cr_env) ;
+  (* eq_lhs := rule.(cr_pat) <[ rule.(cr_sub) ] ; *)
+  eq_lhs := subst_term rule.(cr_sub) rule.(cr_pat) ;
+  eq_rhs := rule.(cr_rep) ;
+  eq_typ := rule.(cr_typ)
+|}.
 
 (** Global declaration **)
 Inductive gdecl :=
