theories/Typing.v
@@ -56,13 +56,13 @@ Section Equations.
       ectx_get Ξ' M = Some (E, ξ') →
       ∃ Ξ'' Δ R,
         Σ E = Some (Ext Ξ'' Δ R) ∧
-        ∀ n rule,
-          nth_error R n = Some rule →
-          let m := length rule.(cr_env) in
+        ∀ n ε,
+          nth_error (map crule_eq R) n = Some ε →
+          let m := length ε.(eq_env) in
           let δ := length Δ in
-          let Θ := ctx_einst ξ (ctx_einst ξ' rule.(cr_env)) in
-          let lhs0 := rule_lhs M ξ' δ rule in
-          let rhs0 := rule_rhs M ξ' δ rule in
+          let Θ := ctx_einst ξ (ctx_einst ξ' ε.(eq_env)) in
+          let lhs0 := rule_lhs M ξ' δ ε in
+          let rhs0 := rule_rhs M ξ' δ ε in
           let lhs := einst (liftn m ξ) lhs0 in
           let rhs := einst (liftn m ξ) rhs0 in
           scoped m lhs0 = true ∧
@@ -87,14 +87,14 @@ Inductive conversion (Γ : ctx) : term → term → Prop :=
       Γ ⊢ const c ξ ≡ einst ξ t
 
 | conv_red :
-    ∀ E Ξ' Δ R M ξ' n rule σ,
+    ∀ E Ξ' Δ R M ξ' n ε σ,
       Σ E = Some (Ext Ξ' Δ R) →
       ectx_get Ξ M = Some (E, ξ') →
-      nth_error R n = Some rule →
+      nth_error (map crule_eq R) n = Some ε →
       let δ := length Δ in
-      let lhs := rule_lhs M ξ' δ rule in
-      let rhs := rule_rhs M ξ' δ rule in
-      let k := length rule.(cr_env) in
+      let lhs := rule_lhs M ξ' δ ε in
+      let rhs := rule_rhs M ξ' δ ε in
+      let k := length ε.(eq_env) in
       scoped k lhs = true →
       scoped k rhs = true →
       Γ ⊢ lhs <[ σ ] ≡ rhs <[ σ ]
@@ -264,14 +264,14 @@ Inductive ewf (Σ : gctx) : ectx → Prop :=
     inst_typing_ Σ Ξ (typing Σ Ξ) ∙ ξ' Ξ' →
     ewf Σ ((E, ξ') :: Ξ).
 
-(** Computation rule typing **)
+(** Equation typing **)
 
-Definition rule_typing Σ Ξ Δ rule :=
-  let k := length rule.(cr_env) in
-  wf Σ Ξ (Δ ,,, rule.(cr_env)) ∧
-  (∃ i, Σ ;; Ξ | Δ ,,, rule.(cr_env) ⊢ rule.(cr_typ) : Sort i) ∧
-  Σ ;; Ξ | Δ ,,, rule.(cr_env) ⊢ rule.(cr_pat) <[ rule.(cr_sub) ] : rule.(cr_typ) ∧
-  Σ ;; Ξ | Δ ,,, rule.(cr_env) ⊢ rule.(cr_rep) : rule.(cr_typ).
+Definition equation_typing Σ Ξ Δ ε :=
+  let k := length ε.(eq_env) in
+  wf Σ Ξ (Δ ,,, ε.(eq_env)) ∧
+  (∃ i, Σ ;; Ξ | Δ ,,, ε.(eq_env) ⊢ ε.(eq_typ) : Sort i) ∧
+  Σ ;; Ξ | Δ ,,, ε.(eq_env) ⊢ ε.(eq_lhs) : ε.(eq_typ) ∧
+  Σ ;; Ξ | Δ ,,, ε.(eq_env) ⊢ ε.(eq_rhs) : ε.(eq_typ).
 
 (** Global environment typing **)
 
@@ -283,7 +283,7 @@ Inductive gwf : gctx → Prop :=
     gwf Σ →
     ewf Σ Ξ →
     wf Σ Ξ Δ →
-    Forall (rule_typing Σ Ξ Δ) R →
+    Forall (equation_typing Σ Ξ Δ) (map crule_eq R) →
     gwf ((c, Ext Ξ Δ R) :: Σ)
 
 | gwf_def c (Σ : gctx) Ξ A t i :
